convert compact to CPS and try out a simple example

src/SaturatedBaseSystem.v
@@ -3,9 +3,9 @@ Require Import Coq.ZArith.ZArith.
 Require Import Coq.Lists.List.
 Local Open Scope Z_scope.
 
-
 Require Import Crypto.Tactics.Algebra_syntax.Nsatz.
 Require Import Crypto.NewBaseSystem.
+Require Import Crypto.Util.LetIn Crypto.Util.CPSUtil.
 Require Import Crypto.Util.Tuple Crypto.Util.ListUtil Crypto.Util.Tactics.
 Local Notation "A ^ n" := (tuple A n) : type_scope.
 
@@ -14,15 +14,17 @@ Local Notation "A ^ n" := (tuple A n) : type_scope.
 Arithmetic on bignums that handles carry bits; this is useful for
 saturated limbs. Compatible with mixed-radix bases.
 
-***)
+ ***)
+
 Section Saturated.
   Context {weight : nat->Z}
           {weight_0 : weight 0%nat = 1}
           {weight_nonzero : forall i, weight i <> 0}
           {weight_multiples : forall i, weight (S i) mod weight i = 0}
-          {add_get_carry: nat->Z -> Z -> (Z * Z)}
-          {add_get_carry_correct : forall i x y,
-              fst (add_get_carry i x y)  = x + y - ((weight (S i) / weight i) * snd (add_get_carry i x y))}
+          (* add_get_carry takes in a number at which to split output *)
+          {add_get_carry: Z ->Z -> Z -> (Z * Z)}
+          {add_get_carry_correct : forall s x y,
+              fst (add_get_carry s x y)  = x + y - s * snd (add_get_carry s x y)}
   .
 
   Definition eval {n} (x : (list Z)^n) : Z :=
@@ -48,31 +50,55 @@ Section Saturated.
   (* Sums a list of integers using carry bits.
      Output : next index, carry, sum
    *)
-  Fixpoint compact_digit n (digit : list Z) : nat * Z * Z :=
+  Fixpoint compact_digit_cps n (digit : list Z) {T} (f:Z * Z->T) :=
   match digit with
-  | nil => (S n, 0, 0)
-  | x :: nil => (S n, 0, x)
+  | nil => f (0, 0)
+  | x :: nil => f (0, x)
   | x :: tl =>
-    let rec := compact_digit n tl in
-    let sum_carry := add_get_carry n x (snd rec) in
-    (S n, snd (fst rec) + snd sum_carry, fst sum_carry)
+    compact_digit_cps n tl (fun rec =>
+      dlet sum_carry := add_get_carry (weight (S n) / weight n) x (snd rec) in
+      dlet carry' := (fst rec + snd sum_carry)%RT in
+    f (carry', fst sum_carry))
   end.
 
-  Definition compact_step (idx_carry:nat*Z) (digit: list Z)
-    : nat * Z * Z :=
-    compact_digit (fst idx_carry) (snd idx_carry::digit).
+  Definition compact_digit n digit := compact_digit_cps n digit id.
+  Lemma compact_digit_id n digit: forall {T} f,
+      @compact_digit_cps n digit T f = f (compact_digit n digit).
+  Proof.
+    induction digit; intros; cbv [compact_digit]; [reflexivity|];
+      simpl compact_digit_cps; break_match; [reflexivity|].
+    rewrite !IHdigit; reflexivity.
+  Qed.
+  Hint Opaque compact_digit : uncps.
+  Hint Rewrite compact_digit_id : uncps.
+
+  Definition compact_step_cps (index:nat) (carry:Z) (digit: list Z)
+    {T} (f:Z * Z->T) :=
+    compact_digit_cps index (carry::digit) f.
+
+  Definition compact_step i c d := compact_step_cps i c d id.
+  Lemma compact_step_id i c d T f :
+    @compact_step_cps i c d T f = f (compact_step i c d).
+  Proof. cbv [compact_step_cps compact_step]; autorewrite with uncps; reflexivity. Qed.
+  Hint Opaque compact_step : uncps.
+  Hint Rewrite compact_step_id : uncps.
   
-  Definition compact {n} (xs : (list Z)^n) : Z * Z^n := 
-    let idx_carry_result := map_with compact_step (0%nat,0) xs in
-    (snd (fst idx_carry_result), snd idx_carry_result).
+  Definition compact_cps {n} (xs : (list Z)^n) {T} (f:Z * Z^n->T) := 
+    mapi_with_cps compact_step_cps 0 xs f.
+
+  Definition compact {n} xs := @compact_cps n xs _ id.
+  Lemma compact_id {n} xs {T} f : @compact_cps n xs T f = f (compact xs).
+  Proof. cbv [compact_cps compact]; autorewrite with uncps; reflexivity. Qed.
 
   Lemma compact_digit_correct i (xs : list Z) :
-    snd (compact_digit i xs)  = sum xs - (weight (S i) / weight i) * snd (fst (compact_digit i xs)).
+    snd (compact_digit i xs)  = sum xs - (weight (S i) / weight i) * (fst (compact_digit i xs)).
   Proof.
-    induction xs; simpl compact_digit in *;
+    induction xs; cbv [compact_digit]; simpl compact_digit_cps;
+      cbv [Let_In];
       repeat match goal with
              | _ => rewrite add_get_carry_correct
              | _ => progress (rewrite ?sum_cons, ?sum_nil in * )
+             | _ => progress (autorewrite with uncps push_id in * )
              | _ => progress (autorewrite with cancel_pair in * )
              | _ => progress break_match; try discriminate
              | _ => progress ring_simplify
@@ -81,17 +107,13 @@ Section Saturated.
              end.
   Qed.
 
-  Lemma fst_fst_compact_step (ic : nat*Z) (digit : list Z) :
-    fst (fst (compact_step ic digit)) = S (fst ic).
-  Proof. destruct digit; reflexivity. Qed.
+  Definition compact_invariant n i (starter rem:Z) (inp : tuple (list Z) n) (out : tuple Z n) :=
+    B.Positional.eval_from weight i out + weight (i + n) * (rem)
+    = eval_from i inp + weight i*starter.
 
-  Definition compact_invariant n (starter rem:nat*Z) (inp : tuple (list Z) n) (out : tuple Z n) :=
-    B.Positional.eval_from weight (fst starter) out + weight (fst starter + n) * (snd rem)
-    = eval_from (fst starter) inp + weight (fst starter)*(snd starter).
-
-  Lemma compact_invariant_holds n starter rem inp out :
-    compact_invariant n (fst (compact_step starter (hd inp))) rem (tl inp) out ->
-    compact_invariant (S n) starter rem inp (append (snd (compact_step starter (hd inp))) out).
+  Lemma compact_invariant_holds n i starter rem inp out :
+    compact_invariant n (S i) (fst (compact_step_cps i starter (hd inp) id)) rem (tl inp) out ->
+    compact_invariant (S n) i starter rem inp (append (snd (compact_step_cps i starter (hd inp) id)) out).
   Proof.
     cbv [compact_invariant B.Positional.eval_from]; intros.
     repeat match goal with
@@ -104,32 +126,41 @@ Section Saturated.
            | _ => (rewrite fst_fst_compact_step in * )
            | _ => progress ring_simplify
            | _ => rewrite ZUtil.Z.mul_div_eq_full by apply weight_nonzero
-           | _ => cbv [compact_step] in *; rewrite compact_digit_correct
+           | _ => cbv [compact_step_cps] in *;
+                    autorewrite with uncps push_id;
+                    rewrite compact_digit_correct
            | _ => progress (autorewrite with natsimplify in * )
            end.
-    rewrite B.Positional.eval_wt_equiv with (wtb := fun i => weight (i + S (fst starter))) by (intros; f_equal; try omega).
+    rewrite B.Positional.eval_wt_equiv with (wtb := fun i0 => weight (i0 + S i)) by (intros; f_equal; try omega).
     nsatz.
   Qed.
 
-  Lemma compact_invariant_base rem : compact_invariant 0 rem rem tt tt.
+  Lemma compact_invariant_base i rem : compact_invariant 0 i rem rem tt tt.
   Proof. cbv [compact_invariant]. simpl. repeat (f_equal; try omega). Qed.
 
   Lemma compact_invariant_end {n} start (input : (list Z)^n):
-    compact_invariant n start (fst (map_with compact_step start input)) input
-                      (snd (map_with compact_step start input)).
+    compact_invariant n 0%nat start (fst (mapi_with_cps compact_step_cps start input id)) input (snd (mapi_with_cps compact_step_cps start input id)).
   Proof.
-    apply (map_with_invariant compact_step compact_invariant
-                              compact_invariant_holds compact_invariant_base).
+    autorewrite with uncps push_id.
+    apply (mapi_with_invariant _ compact_invariant
+                               compact_invariant_holds compact_invariant_base).
   Qed.
 
   Lemma eval_compact {n} (xs : tuple (list Z) n) :
     B.Positional.eval weight (snd (compact xs)) + (weight n * fst (compact xs)) = eval xs.
   Proof.
-    cbv [compact].
-    pose proof (compact_invariant_end (0%nat, 0) xs) as Hinv.
+    pose proof (compact_invariant_end 0 xs) as Hinv.
     cbv [compact_invariant] in Hinv.
     simpl in Hinv. autorewrite with zsimplify natsimplify in Hinv.
-    rewrite eval_from_0, B.Positional.eval_from_0 in Hinv.  apply Hinv.
+    rewrite eval_from_0, B.Positional.eval_from_0 in Hinv; apply Hinv.
   Qed.
 
 End Saturated.
+
+(*
+Definition base10 i := Eval compute in 10^(Z.of_nat i).
+Import ListNotations.
+Eval cbv -[runtime_add runtime_mul Let_In] in
+    (fun adc a0 a1 b0 b1 =>
+       compact (n:=2) (add_get_carry:=adc) (weight:=base10) ([a1;b1],[a0;b0])).
+*)
